update

src/Lending/prajectAave.sol
@@ -1,0 +1,147 @@
+// SPDX-License-Identifier: MIT
+pragma solidity ^0.8.20;
+import "@openzeppelin/ERC20/ERC20.sol";
+import "@openzeppelin/ERC20/IERC20.sol";
+import "@hack/myTokens/myToken.sol";
+//import "";
+import "forge-std/console.sol";
+import "openzeppelin-contracts/contracts/access/Ownable.sol";
+import "math/DSMath.sol";
+import "@hack/libs/safemath.sol";
+import "@hack/Lending/mathematics.sol";
+
+// import "./myAAVE.sol";
+interface ILendingPool {
+    function deposit(
+        address asset,
+        uint256 amount,
+        address onBehalfOf,
+        uint16 referralCode
+    ) external;
+
+    function withdraw(
+        address asset,
+        uint256 amount,
+        address to
+    ) external returns (uint256);
+}
+
+interface IWETHGateway {
+    function depositETH(
+        address lendingPool,
+        address onBehalfOf,
+        uint16 referralCode
+    ) external payable;
+
+    function withdrawETH(
+        address lendingPool,
+        uint256 amount,
+        address onBehalfOf
+    ) external;
+}
+contract Lend is Mathematics, Ownable, DSMath{
+    using SafeMath for uint256;
+    // address public owner;
+    mapping(address=>uint) public userBorrowed;
+    mapping(address=>uint) public userCollateral;
+    //mapping(address=>uint) public depositDAI;
+    // IERC20 public dai;
+    MyToken public bond;
+    uint256 public totalBorrowed;
+    uint256 public totalReserve;
+    uint256 public totalDeposit;
+    uint256 public maxLTV = 4; // 1 = 20%
+    uint256 public ethTreasury;
+    uint256 public totalCollateral;
+    uint256 public baseRate = 20000000000000000;
+    uint256 public fixedAnnuBorrowRate = 300000000000000000;
+    ILendingPool public constant aave = ILendingPool(0xFf795577d9AC8bD7D90Ee22b6C1703490b6512FD);
+    
+    IWETHGateway public constant wethGateway =
+        IWETHGateway(0xA61ca04DF33B72b235a8A28CfB535bb7A5271B70);
+    
+    MyToken public constant dai =
+        MyToken(0xFf795577d9AC8bD7D90Ee22b6C1703490b6512FD);
+    MyToken public constant aDai =
+        MyToken(0xdCf0aF9e59C002FA3AA091a46196b37530FD48a8);
+    MyToken public constant aWeth =
+        MyToken(0x87b1f4cf9BD63f7BBD3eE1aD04E8F52540349347);
+    MyToken private constant weth =
+        MyToken(0xd0A1E359811322d97991E03f863a0C30C2cF029C);
+
+    modifier amountPositive(uint amount){
+        require(amount > 0, "Must be bigger than zero");
+        _;
+    }
+    constructor(address _bond , address initialOwner ) Ownable(initialOwner){
+        bond = MyToken(_bond);
+    }
+    
+    function _sendDaiToAave(uint256 _amount) internal {
+        dai.approve(address(aave), _amount);
+        aave.deposit(address(dai), _amount, address(this), 0);
+    }
+
+    function _withdrawDaiFromAave(uint256 _amount) internal {
+        aave.withdraw(address(dai), _amount, msg.sender);
+    }
+
+    function _sendWethToAave(uint256 _amount) internal {
+        wethGateway.depositETH{value: _amount}(address(aave), address(this), 0);
+    }
+
+    function _withdrawWethFromAave(uint256 _amount) internal {
+        aWeth.approve(address(wethGateway), _amount);
+        wethGateway.withdrawETH(address(aave), _amount, address(this));
+    }
+
+    function bondAsset(uint _amount) external amountPositive(_amount){
+        require(_amount > 0 , "Amount must be biger then zeror");
+        dai.transferFrom(msg.sender,address(this), _amount);
+        totalDeposit += _amount;
+        _sendDaiToAave(_amount);
+        uint bondsToMint = getExp(_amount, getExchangeRate());
+        bond.mint(msg.sender, bondsToMint);
+    } 
+
+    function unbondAsset(uint256 _amount) external {
+        require(_amount > 0 , "Amount must be biger then zeror");
+        require(_amount <= bond.balanceOf(msg.sender), "Not enough bonds!");
+        uint256 daiToReceive = mulExp(_amount, getExchangeRate());
+        totalDeposit -= daiToReceive;
+        bond.burn(msg.sender, _amount);
+        _withdrawDaiFromAave(daiToReceive);
+    }
+
+    //   function addCollateral() external payable {
+    //     require(msg.value != 0, "Cant send 0 ethers");
+    //     usersCollateral[msg.sender] += msg.value;
+    //     totalCollateral += msg.value;
+    //     _sendWethToAave(msg.value);
+    // }
+
+    // function removeCollateral(uint256 _amount) external {
+    //     uint256 wethPrice = uint256(_getLatestPrice());
+    //     uint256 collateral = usersCollateral[msg.sender];
+    //     require(collateral > 0, "Dont have any collateral");
+    //     uint256 borrowed = usersBorrowed[msg.sender];
+    //     uint256 amountLeft = mulExp(collateral, wethPrice).sub(borrowed);
+    //     uint256 amountToRemove = mulExp(_amount, wethPrice);
+    //     require(amountToRemove < amountLeft, "Not enough collateral to remove");
+    //     usersCollateral[msg.sender] -= _amount;
+    //     totalCollateral -= _amount;
+    //     _withdrawWethFromAave(_amount);
+    //     payable(address(this)).transfer(_amount);
+    // }
+    function getExchangeRate() public view returns (uint256) {
+        if (dai.totalSupply() == 0) {
+            return 1000000000000000000;
+        }
+        uint256 cash = getCash();
+        uint256 num = cash.add(totalBorrowed).add(totalReserve);
+        return getExp(num, dai.totalSupply());
+    }
+    function getCash() public view returns (uint256) {
+        return totalDeposit.sub(totalBorrowed);
+    }    
+}
