src/myTokens/myToken.sol
@@ -1,0 +1,16 @@
+// SPDX-License-Identifier: MIT
+pragma solidity ^0.8.0;
+
+import "@openzeppelin/ERC20/ERC20.sol";
+
+contract MyToken is ERC20 {
+    constructor(string memory name, string memory symbol) ERC20(name, symbol) {}
+
+    function mint(address to, uint256 tokenId) external {
+        _mint(to, tokenId);
+    }
+
+        function burn(address to, uint256 tokenId) external {
+        _burn(to, tokenId);
+    }
+}
